Updating stack type with documentation.

stack.v
@@ -1,8 +1,10 @@
-(* 
-The first data type defined in chapter 2 of PFDS.
+(** * The Stack Datatype
+ 
+The Stack is the first data type defined in chapter 2 of PFDS.
 
 Its signature is defined as (in SML):
 
+<<
 signature STACK = 
 sig
   type a Stack
@@ -14,20 +16,43 @@ sig
   val head        :: a Stack -> a
   val tail        :: a Stack -> a Stack
 end
-
+>>
 *)
 
-Require Import Bool.
+(** ----- *)
 
-Inductive stack (T:Set) : Set :=
+Require Import Bool Arith.
+
+(** ** The Implementation *)
+
+(** A stack is either empty, or it is constructed from a series of Cons.
+
+    That is, the list that would be expressed in Haskell as <<[1, 2, 3]>> would
+    be represented herein as [Cons nat 1 (Cons nat 2 (Cons nat 3 (Empty nat)))].
+ *)
+
+Inductive stack (T:Type) : Type :=
   | Empty : stack T
   | Cons : T -> stack T -> stack T.
+
+
+(** An empty stack is represented by the value Empty; therefore, an
+    implementation of isEmpty only needs to match that value.
+ *)
 
 Definition isEmpty T (s : stack T) : bool :=
   match s with
     | Empty => true
-    | _ => false
+    | _     => false
   end.
+
+(** Retrieving the head of the list poses some interesting problems. The book
+    desires an exception be raised for the head of an empty list; however, a
+    formally verified program shouldn't have any erroneous conditions. There
+    is very likely a better way to express this in a definition, but this is
+    day 3 with the language. For now, an option property will suffice. This
+    returns None for an empty list, and Some value for the non-empty stack.
+ *)
 
 Definition head T (s : stack T) : option T :=
   match s with
@@ -41,19 +66,141 @@ Definition tail T (s : stack T) : stack T :=
     | Cons _ s' => s'
   end.
 
-(* Example of empty list. *)
-Eval simpl in Empty nat.
-Eval simpl in isEmpty nat (Empty nat).
+(** In order to allow cons to take a head, the value has to have the option
+    property.
+  *)
 
-(* Example of a list of size 1. *)
-Eval simpl in Cons nat 1 (Empty nat).
-Eval simpl in isEmpty nat (Cons nat 1 (Empty nat)).
+Definition cons T (x : option T) (s : stack T) : stack T :=
+  match x with
+    | None => s
+    | Some x' => Cons T x' s
+  end.
 
+Fixpoint length T (s : stack T) : nat :=
+  match s with
+    | Empty => 0
+    | Cons _ s' => 1 + (length T s')
+  end.
+
+
+(** ----- *)
+(** ** Some examples *)
+
+(** *** The empty stack. *)
+
+Eval simpl in Empty nat. (** <<= Empty nat : stack nat >>*)
+Eval simpl in isEmpty nat (Empty nat). (** <<= true : bool >> *)
+
+(** *** A stack of length 1. *)
+
+Eval simpl in Cons nat 1 (Empty nat). (** <<= Cons nat 1 (Empty nat) : stack nat >> *)
+Eval simpl in isEmpty nat (Cons nat 1 (Empty nat)). (** <<= false : bool >>*)
+
+(** *** Heads or tails? *)
 Definition list1 := Cons nat 1 (Empty nat).
 Definition list2 := Cons nat 2 list1.
+Definition list3 := Cons nat 2 (Cons nat 1 (Empty nat)).
 
-Eval simpl in head nat list1.
-Eval simpl in head nat list2.
-Eval simpl in tail nat list1.
-Eval simpl in tail nat list2.
-Eval simpl in head nat (tail nat list2).
+Eval simpl in head nat list1. (** <<= Some 1 : option nat>> *)
+Eval simpl in head nat list2. (** <<= Some 2 : option nat>> *)
+Eval simpl in tail nat list1. (** <<= Empty nat : stack nat>> *)
+Eval simpl in tail nat list2. (** <<= list1 : stack nat>> *)
+Eval simpl in head nat (tail nat list2). (** <<= Some 1 : option nat>> *)
+Eval simpl in length nat list2. (** <<= 2 : nat>> *)
+Eval simpl in cons nat (head nat list3) (tail nat list3).
+
+Eval simpl in cons nat (head nat list2) (tail nat list2).
+
+(** ----- *)
+(** ** Proving head/tail consistency.
+
+   Theorem: consing the head of a list onto the tail of a list returns the
+   original list. *)
+
+Theorem head_tail_consistency: forall t s,
+  cons t (head t s) (tail t s) = s. 
+Proof.
+  (** Prologue: _dramatis personae_ and split the proof into two cases: one in
+     which the stack is empty, and the other when the stack is not empty. *)
+
+  intros. induction s.
+
+  (** Case 1: the stack is empty. *)
+
+  reflexivity.
+
+  (** Case 2: the stack is not empty. *)
+
+  rewrite <- IHs.
+  reflexivity.
+Qed.
+
+
+(** ** The extracted program (in OCaml) *)
+
+(*
+Extraction "stack.ml" stack isEmpty head tail cons length list1 list2.
+Extraction Language Haskell.
+Extraction "stack.hs" stack isEmpty head tail cons length list1 list2.
+ *)
+
+(**
+<<
+type bool =
+| True
+| False
+
+type nat =
+| O
+| S of nat
+
+type 'a option =
+| Some of 'a
+| None
+
+(** val plus : nat -> nat -> nat **)
+
+let rec plus n m =
+  match n with
+  | O -> m
+  | S p -> S (plus p m)
+
+type 't stack =
+| Empty
+| Cons of 't * 't stack
+
+(** val isEmpty : 'a1 stack -> bool **)
+
+let isEmpty = function
+| Empty -> True
+| Cons (t, s0) -> False
+
+(** val head : 'a1 stack -> 'a1 option **)
+
+let head = function
+| Empty -> None
+| Cons (s', s0) -> Some s'
+
+(** val tail : 'a1 stack -> 'a1 stack **)
+
+let tail = function
+| Empty -> Empty
+| Cons (t, s') -> s'
+
+(** val cons : 'a1 option -> 'a1 stack -> 'a1 stack **)
+
+let cons x s =
+  match x with
+  | Some x' -> Cons (x', s)
+  | None -> s
+
+(** val length : 'a1 stack -> nat **)
+
+let rec length = function
+| Empty -> O
+| Cons (t, s') -> plus (S O) (length s')
+>>
+*)
+
+Eval simpl in tail nat (Empty nat).
+Eval simpl in head nat (Cons nat 1 (Empty nat)).
