Makefile
@@ -1,0 +1,21 @@
+all: stack.html stack.pdf stack.vo
+
+stack.glob: stack.v
+	coqc stack.v
+
+stack.pdf: stack.tex
+	xelatex stack.tex
+
+stack.tex: stack.glob
+	coqdoc -latex stack.v
+
+stack.html: stack.glob
+	coqdoc stack.v
+
+clean:
+	rm -f *.aux *.log *.vo *.glob
+
+nuke: clean
+	rm -f *.html *.tex *.pdf *.hs *.ml* *.css *.sty
+
+.PHONY: all clean nuke
